Make compiler optimise n2w o ORD and CHR o w2n

compiler/bootstrap/translation/to_closProgScript.sml
@@ -66,6 +66,60 @@ val _ = use_long_names:=true;
 (* flat_to_clos                                                               *)
 (* ------------------------------------------------------------------------- *)
 
+val r = translate flat_to_closTheory.dest_pat_pmatch;
+val r = translate flat_to_closTheory.arg1_pmatch;
+val r = translate flat_to_closTheory.arg2_pmatch;
+
+val _ = patternMatchesLib.ENABLE_PMATCH_CASES();
+
+Definition dest_sing_list_def:
+  dest_sing_list x =
+    dtcase x of [y] => SOME y | _ => NONE
+End
+
+val r = translate dest_sing_list_def;
+
+Definition dest_App_Ord_pmatch:
+  dest_App_Ord x =
+    case x of App _ Ord es => dest_sing_list es | _ => NONE
+End
+
+val r = translate dest_App_Ord_pmatch;
+
+Definition dest_App_WordToIntW8_pmatch:
+  dest_App_WordToIntW8 x =
+    case x of App _ (WordToInt W8) es => dest_sing_list es | _ => NONE
+End
+
+val r = translate dest_App_WordToIntW8_pmatch;
+
+Theorem dest_nop_pmatch:
+  dest_nop op e =
+    case op of
+    | WordFromInt W8 =>
+        (dtcase dest_sing_list e of NONE => NONE | SOME e => dest_App_Ord e)
+    | Chr =>
+        (dtcase dest_sing_list e of NONE => NONE | SOME e => dest_App_WordToIntW8 e)
+    | _ => NONE
+Proof
+  CONV_TAC(ONCE_DEPTH_CONV patternMatchesLib.PMATCH_ELIM_CONV)
+  \\ Cases_on ‘op’ \\ fs [flat_to_closTheory.dest_nop_def]
+  THEN1
+   (Cases_on ‘w’ \\ fs []
+    \\ Cases_on ‘e’ \\ fs [dest_sing_list_def]
+    \\ Cases_on ‘t’ \\ fs [dest_sing_list_def]
+    \\ fs [dest_App_Ord_pmatch,dest_App_WordToIntW8_pmatch]
+    \\ CONV_TAC(ONCE_DEPTH_CONV patternMatchesLib.PMATCH_ELIM_CONV)
+    \\ every_case_tac \\ fs [flat_to_closTheory.dest_nop_def,dest_sing_list_def])
+  \\ fs [dest_App_Ord_pmatch,dest_App_WordToIntW8_pmatch]
+  \\ CONV_TAC(ONCE_DEPTH_CONV patternMatchesLib.PMATCH_ELIM_CONV)
+  \\ Cases_on ‘e’ \\ fs [dest_sing_list_def]
+  \\ Cases_on ‘t’ \\ fs [dest_sing_list_def]
+  \\ Cases_on ‘h’ \\ fs [dest_sing_list_def]
+  \\ every_case_tac \\ fs [flat_to_closTheory.dest_nop_def,dest_sing_list_def]
+QED
+
+val r = translate dest_nop_pmatch;
 val r = translate flat_to_closTheory.compile_def;
 
 val flat_to_clos_compile_side = Q.prove(
